```
PRE = (true)
if (a < b) {
	x = a;
} else {
	x = b;
}
POST = (x = min{a, b})
```

- if-Regel:

   - Bedingung: B = `a < b`
   - Positiver Fall: (PRE && B) { x = a; } POST
   - Negativer Fall: (PRE && !B) { x = b; } POST

   - Beweis pos. Fall:
      - Zuweisungsregel: ZP = POST[x/a] = (a = min{a, b})
      - Konsequenzregel: (PRE && B) = (true && (a < b)) = (a < b) => (a = min{a, b}) (letzter Schritt folgt aus math. Minimum). Wir haben gezeigt: (PRE && B) => ZP.

   - Beweis neg. Fall:
      - Zuweisungsregel: ZN = POST[x/b] = (b = min{a, b})
      - Konsequenzregel: (PRE && !B) = (true && !(a < b)) = (a >= b) => (b = min{a, b}) (letzter Schritt folgt aus math. Minimum). Wir haben gezeigt: (PRE && !B) => ZN.